WIP: Refactor RSP and IO.Behavior

Minterop.fst
@@ -47,8 +47,10 @@ instance ml_bool : ml bool = { mldummy = () }
 instance ml_int : ml int = { mldummy = () }
 instance ml_string : ml string = { mldummy = () }
 instance ml_pair t1 t2 {| ml t1 |} {| ml t2 |} : ml (t1 * t2) = { mldummy = () }
-instance ml_mioarrow t1 t2 {| ml t1 |} {| ml t2 |} : ml (t1 -> MIO t2) = { mldummy = () }
-instance ml_miioarrow t1 t2 {| ml t1 |} {| ml t2 |} : ml (t1 -> MIIO t2) = { mldummy = () }
+instance ml_mioarrow t1 t2 {| ml t1 |} {| ml t2 |} : ml (t1 -> MIO t2) =
+  { mldummy = () }
+instance ml_miioarrow t1 t2 {| ml t1 |} {| ml t2 |} : ml (t1 -> MIIO t2) =
+  { mldummy = () }
 
 instance ml_file_descr : ml file_descr = { mldummy = () }
 (** CA: Is this required? **)
@@ -68,43 +70,64 @@ instance ml_file_descr : ml file_descr = { mldummy = () }
 we have 3 importable classes and I don't think they are named very well.
 
 Context:
-One thing we learned is that our import function should not throw errors because we
-need to use it in writing specifications, therefore we want an import function of
-type t1 -> option t2. In the same time, it is much easier to write code using
-exceptions, therefore there is the exn_import, which is just a lift from option to
-exceptions.
+One thing we learned is that our import function should not throw
+errors because we need to use it in writing specifications, therefore
+we want an import function of type t1 -> option t2. In the same time,
+it is much easier to write code using exceptions, therefore there is
+the exn_import, which is just a lift from option to exceptions.
 
 There is a special case for functions. Functions always can be imported, because
 the cast from the strong type to the weak type is done inside the function (?).
-Also, ml types can be always imported safely. Therefore, I added safe_import of type
-t1 -> t2. I am not that happy with the safe_ part in the name. To me import and
-safe_import are both 'safe'.
+Also, ml types can be always imported safely. Therefore, I added
+safe_import of type t1 -> t2. I am not that happy with the safe_ part
+in the name. To me import and safe_import are both 'safe'.
 **)
 
-class exportable (t : Type) = { etype : Type; export : t -> etype; ml_etype : ml etype }
-class importable (t : Type) = { itype : Type; import : itype -> option t; ml_itype : ml itype }
+class exportable (t : Type) =
+  { etype : Type; export : t -> etype; ml_etype : ml etype }
+class importable (t : Type) =
+  { itype : Type; import : itype -> option t; ml_itype : ml itype }
 
-class exn_importable (t : Type) = { eitype : Type; exn_import : eitype -> MIO t; ml_eitype : ml eitype }
-class safe_importable (t : Type) = { sitype : Type; safe_import : sitype -> t; ml_sitype : ml sitype }
+class exn_importable (t : Type) =
+  { eitype : Type; exn_import : eitype -> MIO t; ml_eitype : ml eitype }
+class safe_importable (t : Type) =
+  { sitype : Type; safe_import : sitype -> t; ml_sitype : ml sitype }
 
 let mk_exportable (#t1 t2 : Type) {| ml t2 |} (exp : t1 -> t2) : exportable t1 =
   { etype = t2; export = exp;  ml_etype = solve }
-let mk_importable (t1 #t2 : Type) {| ml t1 |} (imp : t1 -> option t2) : importable t2 =
+
+let mk_importable
+  (t1 #t2 : Type) {| ml t1 |}
+  (imp : t1 -> option t2) :
+  Tot (importable t2) =
   { itype = t1; import = imp; ml_itype = solve }
-let mk_exn_importable (t1 #t2 : Type) {| ml t1 |} (imp : t1 -> MIO t2) : exn_importable t2 =
+
+let mk_exn_importable
+  (t1 #t2 : Type) {| ml t1 |}
+  (imp : t1 -> MIO t2) :
+  Tot (exn_importable t2) =
   { eitype = t1; exn_import = imp; ml_eitype = solve }
-let mk_safe_importable (t1 #t2 : Type) {| ml t1 |} (imp : t1 -> t2) : safe_importable t2 =
+
+let mk_safe_importable
+  (t1 #t2 : Type) {| ml t1 |}
+  (imp : t1 -> t2) :
+  Tot (safe_importable t2) =
   { sitype = t1; safe_import = imp; ml_sitype = solve }
 
 (** Are this two needed? **)
-instance ml_exportable (#t : Type) (d : exportable t) : ml (d.etype) = d.ml_etype
-instance ml_importable (#t : Type) (d : importable t) : ml (d.itype) = d.ml_itype
+instance ml_exportable (#t : Type) (d : exportable t) : ml (d.etype) =
+  d.ml_etype
+instance ml_importable (#t : Type) (d : importable t) : ml (d.itype) =
+  d.ml_itype
 
-instance exportable_ml t {| ml t |} : exportable t = mk_exportable t (fun x -> x)
-instance safe_importable_ml t {| ml t |} : safe_importable t = mk_safe_importable t (fun x -> x)
+instance exportable_ml t {| ml t |} : exportable t =
+  mk_exportable t (fun x -> x)
+instance safe_importable_ml t {| ml t |} : safe_importable t =
+  mk_safe_importable t (fun x -> x)
 
 instance importable_safe_importable t {| d:safe_importable t |} : importable t =
-  mk_importable d.sitype #t #d.ml_sitype (fun (x:d.sitype) -> (Some (safe_import x)) <: option t)
+  mk_importable d.sitype #t #d.ml_sitype
+    (fun (x:d.sitype) -> (Some (safe_import x)) <: option t)
 
 instance exn_importable_importable t {| d:importable t |} : exn_importable t =
   mk_exn_importable d.itype (fun (x:d.itype) ->
@@ -112,16 +135,32 @@ instance exn_importable_importable t {| d:importable t |} : exn_importable t =
     | Some x -> x
     | None -> IO.Effect.throw Contract_failure) <: MIO t)
 
-instance exportable_refinement t {| d:exportable t |} (p : t -> Type0)  : exportable (x:t{p x})
-= mk_exportable (d.etype) export
+instance exportable_refinement
+  t {| d:exportable t |}
+  (p : t -> Type0) :
+  Tot (exportable (x:t{p x})) =
+  mk_exportable (d.etype) export
 
-class checkable (#t:Type) (p : t -> Type0) = { check : (x:t -> b:bool{b ==> p x}) }
-instance general_is_checkeable t (p : t -> bool) : checkable (fun x -> p x) = { check = fun x -> p x }
-class checkable2 (#t1 #t2:Type) (p : t1 -> t2 -> Type0) = { check2 : (x1:t1 -> x2:t2 -> b:bool{b ==> p x1 x2}) }
-instance general_is_checkable2 t1 t2 (p : t1 -> t2 -> bool) : checkable2 (fun x y -> p x y) = { check2 = fun x y -> p x y}
- 
-class checkable4 (#b1 #b2 #b3 #b4:Type) (p : b1 -> b2 -> b3 -> b4 -> Type0) = { check4 : (x1:b1 -> x2:b2 -> x3:b3 -> x4:b4 -> b:bool{b ==> p x1 x2 x3 x4}) }
-instance general_is_checkable4 b1 b2 b3 b4 (p : b1 -> b2 -> b3 -> b4 -> bool) : checkable4 (fun x1 x2 x3 x4 -> p x1 x2 x3 x4) = { check4 = fun x1 x2 x3 x4 -> p x1 x2 x3 x4}
+class checkable (#t:Type) (p : t -> Type0) =
+  { check : (x:t -> b:bool{b ==> p x}) }
+instance general_is_checkeable t (p : t -> bool) : checkable (fun x -> p x) =
+  { check = fun x -> p x }
+class checkable2 (#t1 #t2:Type) (p : t1 -> t2 -> Type0) =
+  { check2 : (x1:t1 -> x2:t2 -> b:bool{b ==> p x1 x2}) }
+instance general_is_checkable2
+  t1 t2 (p : t1 -> t2 -> bool) :
+  Tot (checkable2 (fun x y -> p x y)) =
+  { check2 = fun x y -> p x y}
+
+class checkable4
+  (#b1 #b2 #b3 #b4:Type)
+  (p : b1 -> b2 -> b3 -> b4 -> Type0) =
+  { check4 : (x1:b1 -> x2:b2 -> x3:b3 -> x4:b4 -> b:bool{b ==> p x1 x2 x3 x4}) }
+instance general_is_checkable4
+  b1 b2 b3 b4
+  (p : b1 -> b2 -> b3 -> b4 -> bool) :
+  Tot (checkable4 (fun x1 x2 x3 x4 -> p x1 x2 x3 x4)) =
+  { check4 = fun x1 x2 x3 x4 -> p x1 x2 x3 x4}
 
 instance importable_refinement
   t {| d:importable t |}
@@ -135,17 +174,23 @@ instance importable_refinement
 
 let test_refinement () : MIO (y:int{y = 5}) = exn_import 5
 
-instance exportable_pair t1 t2 {| d1:exportable t1 |} {| d2:exportable t2 |} : exportable (t1 * t2) =
+instance exportable_pair
+  t1 t2 {| d1:exportable t1 |} {| d2:exportable t2 |} :
+  Tot (exportable (t1 * t2)) =
   mk_exportable (d1.etype * d2.etype) (fun (x,y) -> (export x, export y))
 
-instance importable_pair t1 t2 {| d1:importable t1 |} {| d2:importable t2 |} : importable (t1 * t2) =
+instance importable_pair
+  t1 t2 {| d1:importable t1 |} {| d2:importable t2 |} :
+  Tot (importable (t1 * t2)) =
   mk_importable (d1.itype * d2.itype) (fun (x,y) ->
     (match (import x, import y) with
     | (Some x, Some y) -> Some (x, y)
     | _ -> None) <: option (t1 * t2))
 
-instance importable_dpair_refined t1 t2 (p:t1 -> t2 -> Type0)
-  {| d1:importable t1 |} {| d2:importable t2 |} {| d3:checkable2 p |} : importable (x:t1 & y:t2{p x y}) =
+instance importable_dpair_refined
+  t1 t2 (p:t1 -> t2 -> Type0)
+  {| d1:importable t1 |} {| d2:importable t2 |} {| d3:checkable2 p |} :
+  Tot (importable (x:t1 & y:t2{p x y})) =
   mk_importable (d1.itype & d2.itype) #(x:t1 & y:t2{p x y})
     (fun ((x', y')) ->
       (match (import x', import y') with
@@ -156,25 +201,29 @@ instance importable_dpair_refined t1 t2 (p:t1 -> t2 -> Type0)
 let test_dpair_refined () : MIO (a:int & b:int{b = a + 1}) = exn_import (10, 11)
 
 // A typed term in an untyped context
-instance exportable_arrow t1 t2 {| d1:importable t1 |} {| d2:exportable t2 |} : exportable (t1 -> Tot t2)  =
+instance exportable_arrow
+  t1 t2 {| d1:importable t1 |} {| d2:exportable t2 |} :
+  Tot (exportable (t1 -> Tot t2))  =
   mk_exportable (d1.itype -> MIO d2.etype)
-    (fun (f:(t1 -> t2)) -> (fun (x:d1.itype) -> export (f (exn_import x)) <: MIO d2.etype))
- 
-// instance exportable_exarrow t1 t2 {| d1:importable t1 |} {| d2:exportable t2 |} : exportable (t1 -> Ex t2)  =
-//   mk_exportable (d1.itype -> MIO d2.etype)
-//     (fun (f:(t1 -> Ex t2)) -> (fun (x:d1.itype) -> export (f (import x)) <: MIO d2.etype))
+    (fun (f:(t1 -> t2)) ->
+      (fun (x:d1.itype) ->
+        export (f (exn_import x)) <: MIO d2.etype))
 
-instance exportable_mlarrow t1 t2 {| d1:importable t1 |} {| d2:exportable t2 |} : exportable (t1 -> MIO t2)  =
+instance exportable_mlarrow
+  t1 t2 {| d1:importable t1 |} {| d2:exportable t2 |} :
+  Tot (exportable (t1 -> MIO t2)) =
   mk_exportable (d1.itype -> MIO d2.etype)
     (fun (f:(t1 -> MIO t2)) ->
       (fun (x:d1.itype) -> export (f (exn_import x)) <: MIO d2.etype))
 
 // An untyped term in a typed context
-instance importable_mlarrow t1 t2 {| d1:exportable t1 |} {| d2:importable t2 |} : safe_importable (t1 -> MIO t2)  =
+instance importable_mlarrow
+  t1 t2 {| d1:exportable t1 |} {| d2:importable t2 |} :
+  Tot (safe_importable (t1 -> MIO t2)) =
   mk_safe_importable (d1.etype -> MIO d2.itype)
     (fun (f:(d1.etype -> MIO d2.itype)) ->
       (fun (x:t1) -> exn_import (f (export x)) <: MIO t2))
- 
+
 // Example trueish
 let trueish (x:int{x >= 0}) : bool = true
 let trueish' (x:int) : MIO bool = (trueish (exn_import x))
@@ -205,8 +254,11 @@ let incr'' (x:int) : MIO (y:int{p x y}) = exn_import (incr x)
 val incr' : (x:int) -> MIO (y:int{p x y})
 // let incr' = safe_import incr2
 
-instance exportable_purearrow_spec t1 t2 (pre : t1 -> Type0) (post : t1 -> t2 -> Type0)
-  {| d1:importable t1 |} {| d2:exportable t2 |} {| d3:checkable pre |} : exportable ((x:t1) -> Pure t2 (pre x) (post x)) =
+instance exportable_purearrow_spec
+  t1 t2 {| d1:importable t1 |} {| d2:exportable t2 |}
+  (pre : t1 -> Type0) {| d3:checkable pre |}
+  (post : t1 -> t2 -> Type0) :
+  Tot (exportable ((x:t1) -> Pure t2 (pre x) (post x))) =
   mk_exportable (d1.itype -> MIO d2.etype)
     (fun (f:(x:t1 -> Pure t2 (pre x) (post x))) ->
       (fun (x:d1.itype) ->
@@ -434,7 +486,8 @@ instance importable_MIO_pi_IIO
   (pre:t1 -> trace -> Type0) {| d3:checkable2 pre |}
   (post:t1 -> trace -> (m:maybe t2) -> trace -> (r:Type0{Inr? m ==> r}))
   {| d4:checkable4 post |} :
-  Tot (safe_importable (pi:monitorable_prop -> x:t1 -> IIO t2 pi (pre x) (post x))) =
+  Tot (safe_importable (pi:monitorable_prop -> x:t1 ->
+                              IIO t2 pi (pre x) (post x))) =
   mk_safe_importable
     (d1.etype -> MIO d2.itype)
     #(pi:monitorable_prop -> x:t1 -> IIO t2 pi (pre x) (post x))
@@ -460,7 +513,8 @@ instance importable_MIIO_pi_IIO
   (pre:t1 -> trace -> Type0) {| d3:checkable2 pre |}
   (post:t1 -> trace -> (m:maybe t2) -> trace -> (r:Type0{Inr? m ==> r}))
   {| d4:checkable4 post |} :
-  Tot (safe_importable (pi:monitorable_prop -> x:t1 -> IIO t2 pi (pre x) (post x))) =
+  Tot (safe_importable (pi:monitorable_prop -> x:t1 ->
+                               IIO t2 pi (pre x) (post x))) =
   mk_safe_importable
     (d1.etype -> MIIO d2.itype)
     #(pi:monitorable_prop -> x:t1 -> IIO t2 pi (pre x) (post x))
